simulation proof

michael_formal/EFSM.thy
@@ -301,9 +301,6 @@ lemma length_equal_valid: "(length t = length (observe_all e 0 <> t)) = valid e 
 
 type_synonym simulation_relation = "nat \<Rightarrow> nat"
 
-definition simulates_with :: "transition_matrix \<Rightarrow> transition_matrix \<Rightarrow> simulation_relation \<Rightarrow> bool" where
-  "simulates_with m1 m2 H = (\<forall>s r l i s' t. (s', t) |\<in>| possible_steps m1 s r l i \<longrightarrow> (\<exists>t'. (H s', t') |\<in>|possible_steps m2 (H s) r l i))"
-
 definition simulates :: "transition_matrix \<Rightarrow> transition_matrix \<Rightarrow> bool" where
-  "simulates m1 m2 = (\<exists>r. simulates_with m1 m2 r)"
+  "simulates m2 m1 = (\<forall>t. valid_trace m1 t \<longrightarrow> valid_trace m2 t)"
 end
