michael_formal/not4afp/LinkedInLTL.thy
@@ -1,0 +1,122 @@
+theory LinkedInLTL
+imports "../EFSM" "../not4afp/EFSM_LTL"
+
+begin
+abbreviation "outside \<equiv> (0::nat)"
+abbreviation "loggedIn \<equiv> (1::nat)"
+abbreviation "viewDetailed \<equiv> (2::nat)"
+abbreviation "viewSummary \<equiv> (3::nat)"
+abbreviation "pdfDetailed \<equiv> (4::nat)"
+abbreviation "pdfSummary \<equiv> (5::nat)"
+
+definition login :: "transition" where
+"login \<equiv> \<lparr>
+        Label = ''login'',
+        Arity = 1,
+        Guard = [Eq (V (I 1)) (L (Str ''free''))],
+        Outputs = [],
+        Updates = []
+      \<rparr>"
+
+definition viewFriend :: "transition" where
+"viewFriend \<equiv> \<lparr>
+        Label = ''view'',
+        Arity = 3,
+        Guard = [Eq (V (I 1)) (L (Str ''friendID'')), Eq (V (I 2)) (L (Str ''name'')), Eq (V (I 3)) (L (Str ''HM8p''))],
+        Outputs = [L (Str ''friendID''), L (Str ''name''), L (Str ''HM8p'')],
+        Updates = []
+      \<rparr>"
+
+definition viewOther :: "transition" where
+"viewOther \<equiv> \<lparr>
+        Label = ''view'',
+        Arity = 3,
+        Guard = [Eq (V (I 1)) (L (Str ''otherID'')), Eq (V (I 2)) (L (Str ''name'')), Eq (V (I 3)) (L (Str ''4Zof''))],
+        Outputs = [L (Str ''otherID''), L (Str ''name''), L (Str ''4Zof'')],
+        Updates = []
+      \<rparr>"
+
+definition viewOtherOON :: "transition" where
+"viewOtherOON \<equiv> \<lparr>
+        Label = ''view'',
+        Arity = 3,
+        Guard = [Eq (V (I 1)) (L (Str ''otherID'')), Eq (V (I 2)) (L (Str ''OUT_OF_NETWORK'')), Eq (V (I 3)) (L (Str ''MNn5''))],
+        Outputs = [L (Str ''otherID''), L (Str ''OUT_OF_NETWORK''), L (Str ''MNn5'')],
+        Updates = []
+      \<rparr>"
+
+definition viewOtherFuzz :: "transition" where
+"viewOtherFuzz \<equiv> \<lparr>
+        Label = ''view'',
+        Arity = 3,
+        Guard = [Eq (V (I 1)) (L (Str ''otherID'')), Eq (V (I 2)) (L (Str ''name'')), Eq (V (I 3)) (L (Str ''MNn5''))],
+        Outputs = [L (Str ''otherID''), L (Str ''name''), L (Str ''MNn5'')],
+        Updates = []
+      \<rparr>"
+
+definition pdfFriend :: "transition" where
+"pdfFriend \<equiv> \<lparr>
+        Label = ''pdf'',
+        Arity = 3,
+        Guard = [Eq (V (I 1)) (L (Str ''friendID'')), Eq (V (I 2)) (L (Str ''name'')), Eq (V (I 3)) (L (Str ''HM8p''))],
+        Outputs = [],
+        Updates = []
+      \<rparr>"
+
+definition pdfOther :: "transition" where
+"pdfOther \<equiv> \<lparr>
+        Label = ''pdf'',
+        Arity = 3,
+        Guard = [Eq (V (I 1)) (L (Str ''otherID'')), Eq (V (I 2)) (L (Str ''name'')), Eq (V (I 3)) (L (Str ''4Zof''))],
+        Outputs = [],
+        Updates = []
+      \<rparr>"
+
+definition pdfOtherOON :: "transition" where
+"pdfOtherOON \<equiv> \<lparr>
+        Label = ''pdf'',
+        Arity = 3,
+        Guard = [Eq (V (I 1)) (L (Str ''otherID'')), Eq (V (I 2)) (L (Str ''OUT_OF_NETWORK'')), Eq (V (I 3)) (L (Str ''MNn5''))],
+        Outputs = [],
+        Updates = []
+      \<rparr>"
+
+definition linkedIn :: transition_matrix where
+"linkedIn \<equiv> {|
+              ((outside,loggedIn), login),
+              ((loggedIn,viewDetailed), viewFriend),
+              ((loggedIn,viewDetailed), viewOther),
+              ((loggedIn,viewSummary), viewOtherOON),
+              ((loggedIn,viewSummary), viewOtherFuzz),
+              ((viewSummary, pdfSummary), pdfOtherOON),
+              ((viewSummary, pdfDetailed), pdfOther),
+              ((viewDetailed, pdfDetailed), pdfFriend),
+              ((viewDetailed, pdfDetailed), pdfOther)
+         |}"
+
+(*neverDetailed: THEOREM linkedIn |- G(
+(label=login AND ip_1_login_1=String_free) => X(G(
+(label=pdf AND ip_1_view_3=String_otherID) => X(op_1_pdf_1 /= String_detailedPDF)
+)
+);*)
+
+definition login_free :: "property" where
+  "login_free s \<equiv> (event (shd s) = (''login'',  [Str ''free'']))"
+
+definition pdf_other :: "property" where
+  "pdf_other s \<equiv> (let (label, inputs) = event (shd s) in label=''pdf'' \<and> hd inputs = Str ''otherID'')"
+
+definition notDetailedPDF :: "property" where
+  "notDetailedPDF s \<equiv> (hd (output (shd s)) \<noteq> Str ''detailedPDF'')"
+
+(*      G(login_free      =>  X(   G(    pdf_other  =>  X(notDetailedPDF))))*)
+lemma neverDetailed: "(alw login_free impl   (nxt (alw (pdf_other impl (nxt notDetailedPDF))))) 
+     (watch linkedIn i)"
+  oops
+
+lemma neverDetailed_full: "(alw (\<lambda>s. event (shd s) = (''login'',  [Str ''free''])) impl   (nxt (alw ((\<lambda>s. (let (label, inputs) = event (shd s) in label=''pdf'' \<and> hd inputs = Str ''otherID'')) impl (nxt (\<lambda>s. hd (output (shd s)) \<noteq> Str ''detailedPDF'')))))) 
+     (watch linkedIn i)"
+  oops
+
+
+end
